feat: maximality

SeparationLogic/ConvexHull/Andrew_Monotone_Chain.v
@@ -60,6 +60,11 @@ Definition andrew_hull (sorted : list point) : list point :=
 Definition leftdown (p q : point) : Prop :=
   x p < x q \/ (x p = x q /\ y p <= y q).
 
+Lemma point_eq_dec : forall p q : point, {p = q} + {p <> q}.
+Proof.
+  decide equality; apply Z.eq_dec.
+Qed.
+
 Lemma leftdown_refl : forall p,
   leftdown p p.
 Proof.
@@ -827,6 +832,27 @@ Proof.
   exact Hin.
 Qed.
 
+Lemma andrew_lower_chain_in : forall x sorted,
+  In x (andrew_lower_chain sorted) ->
+  In x sorted.
+Proof.
+  intros x sorted Hin.
+  unfold andrew_lower_chain in Hin.
+  apply andrew_chain_in.
+  exact Hin.
+Qed.
+
+Lemma andrew_upper_chain_in : forall x sorted,
+  In x (andrew_upper_chain sorted) ->
+  In x sorted.
+Proof.
+  intros x sorted Hin.
+  unfold andrew_upper_chain in Hin.
+  rewrite in_rev.
+  apply andrew_chain_in.
+  exact Hin.
+Qed.
+
 Lemma graham_scan_inc_preserves_sorted_chain : forall p T,
   Forall (fun q => leftdown q p) T ->
   point_xy_sorted (rev T) ->
@@ -870,6 +896,19 @@ Proof.
     2: exact Hall.
     intros r Hrp.
     exact (leftdown_trans r p q Hrp Hpq).
+Qed.
+
+Lemma graham_scan_inc_tail_forall_leftdown_next :
+  forall p q T,
+  Forall (fun r => leftdown r p) T ->
+  leftdown p q ->
+  Forall (fun r => leftdown r q) T.
+Proof.
+  intros p q T Hall Hpq.
+  eapply Forall_impl.
+  2: exact Hall.
+  intros r Hrp.
+  exact (leftdown_trans r p q Hrp Hpq).
 Qed.
 
 Lemma graham_scan_inc_preserves_rev_sorted_chain : forall p T,
@@ -1112,6 +1151,45 @@ Proof.
   split; [apply Hfirst | apply Hlast]; exact Hq.
 Qed.
 
+Lemma point_xy_sorted_from_fold_left_stack :
+  forall first prefix cur rest,
+  point_xy_sorted_from first (prefix ++ cur :: rest) ->
+  Forall (fun q => leftdown q cur)
+    (fold_left (fun T p => graham_scan_inc p T) prefix [first]).
+Proof.
+  intros first prefix cur rest Hsorted.
+  assert (Hall_prefix : Forall (fun q => leftdown q cur) (first :: prefix)).
+  {
+    pose proof (point_xy_sorted_app_left
+                  (first :: prefix ++ [cur]) rest) as Happ.
+    simpl in Happ.
+    assert (Hsorted_prefix : point_xy_sorted (first :: prefix ++ [cur])).
+    {
+      apply Happ.
+      replace ((prefix ++ [cur]) ++ rest)
+        with (prefix ++ cur :: rest) by (rewrite <- app_assoc; reflexivity).
+      exact Hsorted.
+    }
+    pose proof (point_xy_sorted_all_leftdown_last
+                  first prefix cur Hsorted_prefix) as Hall.
+    rewrite Forall_cons_iff in Hall.
+    destruct Hall as [Hfirst Hall_tail].
+    rewrite Forall_app in Hall_tail.
+    destruct Hall_tail as [Hprefix _].
+    constructor; [exact Hfirst | exact Hprefix].
+  }
+  rewrite Forall_forall in *.
+  intros q Hq.
+  apply Hall_prefix.
+  apply fold_left_graham_scan_inc_in in Hq as [Hq | Hq].
+  - simpl.
+    right.
+    exact Hq.
+  - destruct Hq as [Hq | []].
+    subst q.
+    simpl; left; reflexivity.
+Qed.
+
 Lemma point_xy_rev_sorted_middle_between : forall first middle last,
   point_xy_rev_sorted (last :: (middle ++ [first])) ->
   Forall (fun q => leftdown first q /\ leftdown q last) middle.
@@ -1155,6 +1233,139 @@ Lemma ccw_lower_last_upper : forall first q last r,
   ccw first q last ->
   ccw first last r ->
   ccw q last r.
+Proof.
+  unfold leftdown, x, y, ccw, Record_Geo_Vec.left_than,
+         Record_Geo_Vec.cross_prod, build_vec.
+  simpl; intros; nia.
+Qed.
+
+Lemma point_in_tri_when_baseline_side_flips :
+  forall first q cur a,
+  leftdown first q ->
+  leftdown q cur ->
+  leftdown cur a ->
+  ccw first cur q ->
+  ~ ccw first a q ->
+  point_in_triangle q a cur first.
+Proof.
+  unfold leftdown, x, y, point_in_triangle, ccw,
+         Record_Geo_Vec.left_than, Record_Geo_Vec.left_equal,
+         colinear, Record_Geo_Vec.parallel, at_mid,
+         Record_Geo_Vec.backward_or_perp, Record_Geo_Vec.cross_prod,
+         Record_Geo_Vec.dot_prod, build_vec.
+  simpl; intros; left; repeat split; nia.
+Qed.
+
+Lemma ccw_baseline_side_after_nonleft_turn :
+  forall first q cur a,
+  leftdown first q ->
+  leftdown q cur ->
+  leftdown cur a ->
+  ~ ccw first cur a ->
+  ccw first cur q ->
+  ccw first a q.
+Proof.
+  unfold leftdown, x, y, ccw, Record_Geo_Vec.left_than,
+         Record_Geo_Vec.cross_prod, build_vec.
+  simpl; intros; nia.
+Qed.
+
+Lemma ccw_anchor_side_trans :
+  forall first b cur q,
+  leftdown first q ->
+  leftdown q cur ->
+  leftdown first b ->
+  leftdown b cur ->
+  ccw first b cur ->
+  ccw first cur q ->
+  ccw first b q.
+Proof.
+  intros first b cur q Hfirst_q Hq_cur Hfirst_b Hb_cur Hbcur Hcurq.
+  eapply ccw_anchor_between_trans with (last := cur); eauto.
+Qed.
+
+Lemma baseline_left_equal_not_ccw : forall first last q,
+  Record_Geo_Vec.left_equal (build_vec first last) (build_vec first q) ->
+  ~ ccw first last q.
+Proof.
+  unfold ccw, Record_Geo_Vec.left_than, Record_Geo_Vec.left_equal,
+         Record_Geo_Vec.cross_prod, build_vec.
+  simpl; intros; nia.
+Qed.
+
+Lemma not_ccw_baseline_left_equal : forall first last q,
+  ~ ccw first last q ->
+  Record_Geo_Vec.left_equal (build_vec first last) (build_vec first q).
+Proof.
+  unfold ccw, Record_Geo_Vec.left_than, Record_Geo_Vec.left_equal,
+         Record_Geo_Vec.cross_prod, build_vec.
+  simpl; intros; nia.
+Qed.
+
+Lemma opposite_left_equal_colinear : forall p q r,
+  Record_Geo_Vec.left_equal (build_vec p r) (build_vec p q) ->
+  Record_Geo_Vec.left_equal (build_vec r p) (build_vec r q) ->
+  colinear q p r.
+Proof.
+  unfold Record_Geo_Vec.left_equal, Record_Geo_Vec.left_than,
+         colinear, Record_Geo_Vec.parallel, Record_Geo_Vec.cross_prod,
+         build_vec.
+  simpl; intros; nia.
+Qed.
+
+Lemma leftdown_colinear_between_at_mid : forall p q r,
+  colinear q p r ->
+  leftdown p q ->
+  leftdown q r ->
+  at_mid q p r.
+Proof.
+  unfold colinear, Record_Geo_Vec.parallel, leftdown,
+         at_mid, Record_Geo_Vec.backward_or_perp,
+         Record_Geo_Vec.cross_prod, Record_Geo_Vec.dot_prod, build_vec.
+  simpl.
+  intros [px py] [qx qy] [rx ry] Hcol Hpq Hqr.
+  simpl in *.
+  destruct Hpq as [Hpqx | [Hpqx Hpqy]];
+  destruct Hqr as [Hqrx | [Hqrx Hqry]].
+  - assert (Hcol' :
+        (px - qx) * (ry - qy) = (py - qy) * (rx - qx)) by nia.
+    assert (Hdot :
+            (rx - qx) *
+              ((px - qx) * (rx - qx) +
+               (py - qy) * (ry - qy)) =
+            (px - qx) *
+              ((rx - qx) * (rx - qx) +
+               (ry - qy) * (ry - qy))).
+    {
+      replace ((rx - qx) *
+                 ((px - qx) * (rx - qx) +
+                  (py - qy) * (ry - qy)))
+        with ((px - qx) * (rx - qx) * (rx - qx) +
+              (py - qy) * (rx - qx) * (ry - qy)) by ring.
+      rewrite <- Hcol'.
+      ring.
+    }
+    pose proof (Z.square_nonneg (rx - qx)) as Hsqx.
+    pose proof (Z.square_nonneg (ry - qy)) as Hsqy.
+    assert (0 <= (rx - qx) * (rx - qx) +
+                 (ry - qy) * (ry - qy)) by nia.
+    nia.
+  - assert (ry = qy) by nia.
+    nia.
+  - assert (py = qy) by nia.
+    nia.
+  - nia.
+Qed.
+
+Lemma upper_point_popped_by_lower_point : forall first t q a last,
+  leftdown first t ->
+  leftdown t q ->
+  leftdown q a ->
+  leftdown a last ->
+  ~ ccw first last t ->
+  ccw first last q ->
+  ~ ccw first last a ->
+  ~ ccw t q a.
 Proof.
   unfold leftdown, x, y, ccw, Record_Geo_Vec.left_than,
          Record_Geo_Vec.cross_prod, build_vec.
@@ -1425,6 +1636,85 @@ Proof.
   simpl.
   exists (rev stack_mid).
   reflexivity.
+Qed.
+
+Lemma andrew_lower_chain_as_graham_scan :
+  forall first middle last,
+  andrew_lower_chain (first :: middle ++ [last]) =
+  rev (graham_scan (rev (first :: middle ++ [last]))).
+Proof.
+  intros first middle last.
+  unfold andrew_lower_chain, andrew_chain, andrew_scan_stack.
+  simpl.
+  rewrite fold_left_graham_scan_inc_cons.
+  reflexivity.
+Qed.
+
+Lemma andrew_upper_chain_as_graham_scan :
+  forall first middle last,
+  andrew_upper_chain (first :: middle ++ [last]) =
+  rev (graham_scan (first :: middle ++ [last])).
+Proof.
+  intros first middle last.
+  unfold andrew_upper_chain, andrew_chain, andrew_scan_stack.
+  simpl.
+  rewrite rev_app_distr.
+  simpl.
+  rewrite fold_left_graham_scan_inc_cons.
+  replace (rev (last :: rev middle ++ [first]))
+    with (first :: middle ++ [last]).
+  2: {
+    simpl.
+    rewrite rev_app_distr.
+    simpl.
+    rewrite rev_involutive.
+    reflexivity.
+  }
+  reflexivity.
+Qed.
+
+Lemma andrew_lower_chain_stack_shape :
+  forall first middle last lower_mid,
+  andrew_lower_chain (first :: middle ++ [last]) =
+    first :: lower_mid ++ [last] ->
+  andrew_scan_stack (first :: middle ++ [last]) =
+    last :: rev lower_mid ++ [first].
+Proof.
+  intros first middle last lower_mid Hchain.
+  unfold andrew_lower_chain, andrew_chain in Hchain.
+  apply (f_equal (@rev point)) in Hchain.
+  rewrite rev_involutive in Hchain.
+  simpl in Hchain.
+  rewrite rev_app_distr in Hchain.
+  simpl in Hchain.
+  exact Hchain.
+Qed.
+
+Lemma andrew_upper_chain_stack_shape :
+  forall first middle last upper_mid,
+  andrew_upper_chain (first :: middle ++ [last]) =
+    last :: upper_mid ++ [first] ->
+  andrew_scan_stack (rev (first :: middle ++ [last])) =
+    first :: rev upper_mid ++ [last].
+Proof.
+  intros first middle last upper_mid Hchain.
+  unfold andrew_upper_chain, andrew_chain in Hchain.
+  apply (f_equal (@rev point)) in Hchain.
+  rewrite rev_involutive in Hchain.
+  simpl in Hchain.
+  rewrite rev_app_distr in Hchain.
+  simpl in Hchain.
+  rewrite rev_app_distr in Hchain.
+  simpl in Hchain.
+  replace (rev (first :: middle ++ [last]))
+    with (last :: rev middle ++ [first]).
+  2: {
+    simpl.
+    rewrite rev_app_distr.
+    simpl.
+    reflexivity.
+  }
+  exact Hchain.
 Qed.
 
 Lemma removelast_snoc : forall {A : Type} (l : list A) x,
@@ -1843,6 +2133,175 @@ Proof.
     + apply Forall_nil.
 Qed.
 
+Lemma point_in_hull_member_weak : forall p CH q,
+  weak_rev_ccw_list p CH ->
+  In q CH ->
+  point_in_hull q (p :: CH).
+Proof.
+  intros p CH.
+  induction CH as [| a CH IH]; intros q Hweak Hin.
+  - contradiction.
+  - destruct Hin as [Hq | Hin].
+    + subst q.
+      apply gs_point_in_hull_new_head.
+      exact Hweak.
+    + destruct CH as [| b CH'].
+      * contradiction.
+      * apply point_in_hull_cons_weak.
+        -- exact Hweak.
+        -- apply IH.
+           ++ exact (proj2 Hweak).
+           ++ exact Hin.
+Qed.
+
+Lemma point_in_hull_pop_weak : forall p a b c l q,
+  g_rev_ccw_list p (c :: b :: a :: l) ->
+  ~ ccw a b c ->
+  point_in_hull q (p :: c :: b :: a :: l) ->
+  point_in_hull q (p :: c :: a :: l).
+Proof.
+  intros p a b c l q Hweak Hn Hinh.
+  assert (Hmax : is_max_hull' p (c :: b :: a :: l) [q]).
+  {
+    unfold is_max_hull'.
+    rewrite Forall_cons_iff.
+    split; [exact Hinh | apply Forall_nil].
+  }
+  pose proof (is_max_hull'_pop'_g p a b c l [q]
+                Hweak Hn Hmax) as Hmax'.
+  unfold is_max_hull' in Hmax'.
+  rewrite Forall_cons_iff in Hmax'.
+  exact (proj1 Hmax').
+Qed.
+
+Lemma graham_scan_inc_preserves_cover_disj :
+  forall first a C L,
+  weak_rev_ccw_list first (a :: C) ->
+  Forall
+    (fun q =>
+       point_in_hull q (first :: a :: C) \/
+       ccw first a q)
+    L ->
+  Forall
+    (fun q =>
+       point_in_hull q
+         (first :: removelast (graham_scan_inc a (C ++ [first]))) \/
+       ccw first a q)
+    L.
+Proof.
+  intros first a C.
+  induction C as [| b C IH]; intros L Hweak Hcover.
+  - simpl.
+    exact Hcover.
+  - destruct C as [| c C'].
+    + simpl in *.
+      destruct (ccw_dec first b a) as [Hccw | Hnccw].
+      * simpl.
+        exact Hcover.
+      * rewrite Forall_forall in *.
+        intros q Hq.
+        specialize (Hcover q Hq) as [Hinh | Habove].
+        -- left.
+           apply (gs_point_in_hull_pop_single first a b q).
+           ++ simpl in Hweak.
+              destruct Hweak as [Hfor _].
+              rewrite Forall_g_rev_ccw_cons_iff in Hfor.
+              exact (proj1 Hfor).
+           ++ exact Hnccw.
+           ++ exact Hinh.
+        -- right.
+           exact Habove.
+    + simpl in *.
+      destruct (ccw_dec c b a) as [Hccw | Hnccw].
+      * simpl.
+        assert (Htail :
+          match C' ++ [first] with
+          | [] => []
+          | _ :: _ => c :: removelast (C' ++ [first])
+          end = c :: C').
+        {
+          destruct (C' ++ [first]) as [| h t] eqn:Happ.
+          - destruct C'; simpl in Happ; discriminate.
+          - rewrite <- Happ.
+            rewrite removelast_snoc.
+            reflexivity.
+        }
+        rewrite Htail.
+        exact Hcover.
+      * apply IH.
+        -- pose proof (weak_rev_ccw_list_remove_middle
+                         first [a] [b] (c :: C') Hweak) as Hweak'.
+           simpl in Hweak'.
+           exact Hweak'.
+        -- rewrite Forall_forall in *.
+           intros q Hq.
+           specialize (Hcover q Hq) as [Hinh | Habove].
+           ++ left.
+              eapply point_in_hull_pop_weak.
+              ** exact Hweak.
+              ** exact Hnccw.
+              ** exact Hinh.
+           ++ right.
+              exact Habove.
+Qed.
+
+Lemma lower_cover_push_candidate :
+  forall first cur a C L,
+  weak_rev_ccw_list first (a :: cur :: C) ->
+  leftdown cur a ->
+  Forall (fun q => leftdown first q /\ leftdown q cur) L ->
+  Forall
+    (fun q =>
+       point_in_hull q (first :: cur :: C) \/
+       ccw first cur q)
+    L ->
+  Forall
+    (fun q =>
+       point_in_hull q (first :: a :: cur :: C) \/
+       ccw first a q)
+    L.
+Proof.
+  intros first cur a C L Hweak Hcur_a Hbetween Hcover.
+  rewrite Forall_forall in *.
+  intros q Hq.
+  specialize (Hcover q Hq) as [Hinh | Habove_old].
+  - left.
+    eapply point_in_hull_cons_weak.
+    + exact Hweak.
+    + exact Hinh.
+  - destruct (ccw_dec first a q) as [Habove_new | Hnot_above_new].
+    + right.
+      exact Habove_new.
+    + left.
+      simpl.
+      left.
+      specialize (Hbetween q Hq) as [Hfirst_q Hq_cur].
+      eapply point_in_tri_when_baseline_side_flips; eauto.
+Qed.
+
+Lemma lower_cover_step :
+  forall first cur a C L,
+  weak_rev_ccw_list first (a :: cur :: C) ->
+  leftdown cur a ->
+  Forall (fun q => leftdown first q /\ leftdown q cur) L ->
+  Forall
+    (fun q =>
+       point_in_hull q (first :: cur :: C) \/
+       ccw first cur q)
+    L ->
+  Forall
+    (fun q =>
+       point_in_hull q
+         (first :: removelast (graham_scan_inc a ((cur :: C) ++ [first]))) \/
+       ccw first a q)
+    L.
+Proof.
+  intros first cur a C L Hweak Hcur_a Hbetween Hcover.
+  apply graham_scan_inc_preserves_cover_disj.
+  - exact Hweak.
+  - eapply lower_cover_push_candidate; eauto.
+Qed.
+
 Lemma g_ccw_to_g_rev_ccw_rev : forall p q r,
   g_ccw p r q ->
   g_rev_ccw p q r.
@@ -1905,6 +2364,76 @@ Proof.
   - apply g_ccw_list_to_g_rev_ccw_list_rev.
     apply g_ccw_ccw_list.
     exact Hlist.
+Qed.
+
+Lemma weak_rev_ccw_list_of_sorted_clean_stack : forall first T,
+  point_xy_sorted (rev (T ++ [first])) ->
+  rev_consec_ccw (T ++ [first]) ->
+  weak_rev_ccw_list first T.
+Proof.
+  intros first T Hsorted Hcon.
+  assert (Hsorted' : point_xy_sorted (first :: rev T)).
+  {
+    rewrite rev_app_distr in Hsorted.
+    simpl in Hsorted.
+    exact Hsorted.
+  }
+  assert (Hcon' : consec_ccw (first :: rev T)).
+  {
+    replace (first :: rev T) with (rev (T ++ [first])).
+    2: {
+      rewrite rev_app_distr.
+      reflexivity.
+    }
+    apply gs_rev_consec_ccw_rev_consec.
+    exact Hcon.
+  }
+  assert (Hleft : leftmost first (rev T)).
+  {
+    simpl in Hsorted'.
+    apply point_xy_sorted_from_leftdown_head.
+    exact Hsorted'.
+  }
+  assert (Hconv : ccw_convex (first :: rev T)).
+  {
+    simpl in Hsorted'.
+    apply xy_consec_ccw_to_ccw_convex; assumption.
+  }
+  pose proof (ccw_convex_tail_sort_rev first (rev T) Hleft Hconv)
+    as [_ Hweak].
+  rewrite rev_involutive in Hweak.
+  exact Hweak.
+Qed.
+
+Lemma graham_scan_inc_removelast_preserves_bottom : forall p stack bottom,
+  graham_scan_inc p (stack ++ [bottom]) =
+    removelast (graham_scan_inc p (stack ++ [bottom])) ++ [bottom].
+Proof.
+  intros p stack bottom.
+  destruct (graham_scan_inc_preserves_bottom p stack bottom)
+    as [stack' Hstack].
+  rewrite Hstack.
+  rewrite removelast_snoc.
+  reflexivity.
+Qed.
+
+Lemma graham_scan_inc_clean_stack_weak :
+  forall first a stack,
+  point_xy_sorted (rev (stack ++ [first])) ->
+  Forall (fun q => leftdown q a) (stack ++ [first]) ->
+  rev_consec_ccw (stack ++ [first]) ->
+  weak_rev_ccw_list first
+    (removelast (graham_scan_inc a (stack ++ [first]))).
+Proof.
+  intros first a stack Hsorted Hall Hcon.
+  pose proof (graham_scan_inc_removelast_preserves_bottom a stack first)
+    as Hshape.
+  eapply weak_rev_ccw_list_of_sorted_clean_stack.
+  - rewrite <- Hshape.
+    apply graham_scan_inc_preserves_sorted_chain; assumption.
+  - rewrite <- Hshape.
+    apply graham_scan_inc_rev_consec.
+    exact Hcon.
 Qed.
 
 Lemma rev_consec_ccw_of_consec_rev : forall l,
@@ -2047,6 +2576,46 @@ Proof.
     exact (proj1 (Hupper_between q Hq)).
 Qed.
 
+Lemma andrew_lower_mid_below_baseline :
+  forall first middle last lower_mid,
+  point_xy_sorted (first :: middle ++ [last]) ->
+  andrew_lower_chain (first :: middle ++ [last]) =
+    first :: lower_mid ++ [last] ->
+  forall q, In q lower_mid -> ccw first q last.
+Proof.
+  intros first middle last lower_mid Hsorted Hlower q Hq.
+  pose proof (andrew_lower_chain_ccw_convex
+                (first :: middle ++ [last]) Hsorted) as Hlower_conv.
+  rewrite Hlower in Hlower_conv.
+  simpl in Hlower_conv.
+  destruct Hlower_conv as [Hlower_list _].
+  rewrite ccw_list_app_iff in Hlower_list.
+  destruct Hlower_list as [_ [_ Hcross]].
+  apply Hcross; [exact Hq | simpl; auto].
+Qed.
+
+Lemma andrew_upper_mid_above_baseline :
+  forall first middle last upper_mid,
+  point_xy_sorted (first :: middle ++ [last]) ->
+  andrew_upper_chain (first :: middle ++ [last]) =
+    last :: upper_mid ++ [first] ->
+  forall q, In q upper_mid -> ccw first last q.
+Proof.
+  intros first middle last upper_mid Hsorted Hupper q Hq.
+  pose proof (andrew_upper_chain_ccw_convex
+                (first :: middle ++ [last]) Hsorted) as Hupper_conv.
+  rewrite Hupper in Hupper_conv.
+  pose proof (ccw_convex_app_comm (last :: upper_mid) [first]
+                Hupper_conv) as Hupper_rot.
+  simpl in Hupper_rot.
+  destruct Hupper_rot as [Hupper_first_list _].
+  simpl in Hupper_first_list.
+  destruct Hupper_first_list as [Hforall _].
+  rewrite Forall_ccw_forall in Hforall.
+  apply Hforall.
+  exact Hq.
+Qed.
+
 Lemma andrew_merged_triangle_max_to_edges :
   forall first middle last lower_mid upper_mid,
   point_xy_sorted (first :: middle ++ [last]) ->
@@ -2078,6 +2647,1667 @@ Proof.
   - eapply andrew_ccw_merge_leftmost; eauto.
   - exact Hconv.
   - exact Hmax.
+Qed.
+
+Fixpoint point_left_of_path_edges_from
+    (q prev : point) (path : list point) : Prop :=
+  match path with
+  | p :: rest =>
+      Record_Geo_Vec.left_equal (build_vec prev p) (build_vec prev q) /\
+      point_left_of_path_edges_from q p rest
+  | [] => True
+  end.
+
+Definition point_left_of_path_edges (q : point) (path : list point) : Prop :=
+  match path with
+  | prev :: rest => point_left_of_path_edges_from q prev rest
+  | [] => True
+  end.
+
+Lemma point_left_of_path_edges_cons :
+  forall q p r rest,
+  Record_Geo_Vec.left_equal (build_vec p r) (build_vec p q) ->
+  point_left_of_path_edges q (r :: rest) ->
+  point_left_of_path_edges q (p :: r :: rest).
+Proof.
+  intros q p r rest Hedge Hpath.
+  simpl.
+  split; assumption.
+Qed.
+
+Lemma point_left_of_path_edges_tail :
+  forall q p r rest,
+  point_left_of_path_edges q (p :: r :: rest) ->
+  point_left_of_path_edges q (r :: rest).
+Proof.
+  intros q p r rest Hpath.
+  simpl in Hpath.
+  exact (proj2 Hpath).
+Qed.
+
+Lemma left_equal_pop_shortcut :
+  forall q p t s,
+  ~ ccw s t p ->
+  Record_Geo_Vec.left_equal (build_vec p t) (build_vec p q) ->
+  Record_Geo_Vec.left_equal (build_vec t s) (build_vec t q) ->
+  Record_Geo_Vec.left_equal (build_vec p s) (build_vec p q).
+Proof.
+  unfold ccw, Record_Geo_Vec.left_than, Record_Geo_Vec.left_equal,
+         Record_Geo_Vec.cross_prod, build_vec.
+  simpl; intros; nia.
+Qed.
+
+Lemma point_left_of_path_edges_pop_middle :
+  forall q p t s rest,
+  ~ ccw s t p ->
+  point_left_of_path_edges q (p :: t :: s :: rest) ->
+  point_left_of_path_edges q (p :: s :: rest).
+Proof.
+  intros q p t s rest Hnccw Hpath.
+  simpl in Hpath |- *.
+  destruct Hpath as [Hpt [Hts Htail]].
+  split.
+  - eapply left_equal_pop_shortcut; eauto.
+  - exact Htail.
+Qed.
+
+Lemma point_left_of_path_edges_graham_scan_inc_cleanup :
+  forall q p T,
+  point_left_of_path_edges q (p :: T) ->
+  point_left_of_path_edges q (graham_scan_inc p T).
+Proof.
+  intros q p T.
+  revert p.
+  induction T as [| t T IH]; intros p Hpath; simpl in *.
+  - exact I.
+  - destruct T as [| s rest].
+    + exact Hpath.
+    + destruct (ccw_dec s t p) as [_ | Hnccw].
+      * exact Hpath.
+      * apply IH.
+        eapply point_left_of_path_edges_pop_middle; eauto.
+Qed.
+
+Lemma Forall_point_left_of_path_edges_graham_scan_inc_cleanup :
+  forall L p T,
+  Forall (fun q => point_left_of_path_edges q (p :: T)) L ->
+  Forall (fun q => point_left_of_path_edges q (graham_scan_inc p T)) L.
+Proof.
+  intros L p T Hcover.
+  eapply Forall_impl.
+  2: exact Hcover.
+  intros q Hq.
+  apply point_left_of_path_edges_graham_scan_inc_cleanup.
+  exact Hq.
+Qed.
+
+Lemma left_equal_push_support_lower :
+  forall q s t a,
+  leftdown s t ->
+  leftdown q t ->
+  leftdown t a ->
+  ccw s t a ->
+  Record_Geo_Vec.left_equal (build_vec t s) (build_vec t q) ->
+  Record_Geo_Vec.left_equal (build_vec a t) (build_vec a q).
+Proof.
+  unfold leftdown, ccw, Record_Geo_Vec.left_than,
+         Record_Geo_Vec.left_equal, Record_Geo_Vec.cross_prod, build_vec,
+         x, y.
+  simpl.
+  intros [qx qy] [sx sy] [tx ty] [ax ay] Hst Hqt Hta Hturn Hedge.
+  simpl in *.
+  set (dx := tx - sx) in *.
+  set (dy := ty - sy) in *.
+  set (ux := ax - tx) in *.
+  set (uy := ay - ty) in *.
+  set (vx := qx - tx) in *.
+  set (vy := qy - ty) in *.
+  assert (Hturn' : dx * uy - dy * ux > 0) by (subst; ring_simplify; nia).
+  assert (Hedge' : dx * vy - dy * vx >= 0) by (subst; ring_simplify; nia).
+  assert (Hdx : dx > 0).
+  {
+    destruct Hst as [Hst | [Hstx Hsty]];
+    destruct Hta as [Hta | [Htax Htay]]; subst; nia.
+  }
+  assert (Hux_nonneg : 0 <= ux).
+  {
+    destruct Hta as [Hta | [Htax Htay]]; subst; nia.
+  }
+  assert (Hvx_nonpos : vx <= 0).
+  {
+    destruct Hqt as [Hqt | [Hqtx Hqty]]; subst; nia.
+  }
+  assert (Hgoal_shift : ux * vy - uy * vx >= 0).
+  {
+    destruct (Z_lt_ge_dec 0 ux) as [Hux_pos | Hux_zeroish].
+    - destruct Hqt as [Hvx_neg | [Hvx_eq Hvy_nonpos]].
+      + assert (Hid :
+          dx * (ux * vy - uy * vx) =
+          ux * (dx * vy - dy * vx) -
+          vx * (dx * uy - dy * ux)) by ring.
+        assert (0 <= ux * (dx * vy - dy * vx)) by nia.
+        assert (0 <= - vx * (dx * uy - dy * ux)) by nia.
+        nia.
+      + assert (vx = 0) by (subst; nia).
+        assert (vy = 0) by nia.
+        nia.
+    - assert (ux = 0) by nia.
+      subst ux.
+      destruct Hta as [Hta | [Htax Htay]]; [nia |].
+      nia.
+  }
+  subst dx dy ux uy vx vy.
+  ring_simplify in Hgoal_shift.
+  nia.
+Qed.
+
+Lemma left_equal_pop_support_lower :
+  forall q s t a,
+  leftdown s q ->
+  leftdown q t ->
+  leftdown s t ->
+  leftdown t a ->
+  ~ ccw s t a ->
+  Record_Geo_Vec.left_equal (build_vec t s) (build_vec t q) ->
+  Record_Geo_Vec.left_equal (build_vec a s) (build_vec a q).
+Proof.
+  unfold leftdown, ccw, Record_Geo_Vec.left_than,
+         Record_Geo_Vec.left_equal, Record_Geo_Vec.cross_prod, build_vec,
+         x, y.
+  simpl.
+  intros [qx qy] [sx sy] [tx ty] [ax ay] Hsq Hqt Hst Hta Hturn Hedge.
+  simpl in *.
+  set (dx := tx - sx) in *.
+  set (dy := ty - sy) in *.
+  set (ux := ax - tx) in *.
+  set (uy := ay - ty) in *.
+  set (vx := qx - tx) in *.
+  set (vy := qy - ty) in *.
+  assert (Hturn' : dx * uy - dy * ux <= 0) by (subst; ring_simplify; nia).
+  assert (Hedge' : dx * vy - dy * vx >= 0) by (subst; ring_simplify; nia).
+  assert (Hdx : dx >= 0).
+  {
+    destruct Hst as [Hst | [Hstx Hsty]]; subst; nia.
+  }
+  assert (Hux_nonneg : 0 <= ux).
+  {
+    destruct Hta as [Hta | [Htax Htay]]; subst; nia.
+  }
+  assert (Hvx_nonpos : vx <= 0).
+  {
+    destruct Hqt as [Hqt | [Hqtx Hqty]]; subst; nia.
+  }
+  assert (Hsv_nonneg : 0 <= vx + dx).
+  {
+    destruct Hsq as [Hsq | [Hsqx Hsqy]]; subst; nia.
+  }
+  assert (Hgoal_shift : (ux + dx) * (vy + dy) - (uy + dy) * (vx + dx) >= 0).
+  {
+    assert (Hid :
+      dx * ((ux + dx) * (vy + dy) - (uy + dy) * (vx + dx)) =
+      (ux + dx) * (dx * vy - dy * vx) -
+      (vx + dx) * (dx * uy - dy * ux)) by ring.
+    destruct (Z.eq_dec dx 0) as [Hdx0 | Hdx_ne].
+    - subst dx.
+      assert (vx = 0) by nia.
+      subst vx.
+      destruct Hst as [Hst | [Hstx Hsty]]; [nia |].
+      destruct Hsq as [Hsq | [Hsqx Hsqy]]; [nia |].
+      destruct Hqt as [Hqt | [Hqtx Hqty]]; [nia |].
+      subst; nia.
+    - assert (Hdx_pos : dx > 0) by nia.
+      assert (0 <= (ux + dx) * (dx * vy - dy * vx)) by nia.
+      assert (0 <= - (vx + dx) * (dx * uy - dy * ux)) by nia.
+      nia.
+  }
+  subst dx dy ux uy vx vy.
+  ring_simplify in Hgoal_shift.
+  nia.
+Qed.
+
+Lemma left_equal_push_support_upper :
+  forall q s t a,
+  leftdown t s ->
+  leftdown t q ->
+  leftdown a t ->
+  ccw s t a ->
+  Record_Geo_Vec.left_equal (build_vec t s) (build_vec t q) ->
+  Record_Geo_Vec.left_equal (build_vec a t) (build_vec a q).
+Proof.
+  unfold leftdown, ccw, Record_Geo_Vec.left_than,
+         Record_Geo_Vec.left_equal, Record_Geo_Vec.cross_prod, build_vec,
+         x, y.
+  simpl.
+  intros [qx qy] [sx sy] [tx ty] [ax ay] Hts Htq Hat Hturn Hedge.
+  simpl in *.
+  set (dx := sx - tx) in *.
+  set (dy := sy - ty) in *.
+  set (ux := tx - ax) in *.
+  set (uy := ty - ay) in *.
+  set (vx := qx - tx) in *.
+  set (vy := qy - ty) in *.
+  assert (Hturn' : dx * uy - dy * ux > 0) by (subst; ring_simplify; nia).
+  assert (Hedge' : dx * vy - dy * vx <= 0) by (subst; ring_simplify; nia).
+  assert (Hdx : dx > 0).
+  {
+    destruct Hts as [Hts | [Htsx Htsy]];
+    destruct Hat as [Hat | [Hatx Haty]]; subst; nia.
+  }
+  assert (Hux_nonneg : 0 <= ux).
+  {
+    destruct Hat as [Hat | [Hatx Haty]]; subst; nia.
+  }
+  assert (Hvx_nonneg : 0 <= vx).
+  {
+    destruct Htq as [Htq | [Htqx Htqy]]; subst; nia.
+  }
+  assert (Hgoal_shift : ux * vy - uy * vx <= 0).
+  {
+    destruct (Z_lt_ge_dec 0 ux) as [Hux_pos | Hux_zeroish].
+    - assert (Hid :
+        dx * (ux * vy - uy * vx) =
+        ux * (dx * vy - dy * vx) -
+        vx * (dx * uy - dy * ux)) by ring.
+      assert (ux * (dx * vy - dy * vx) <= 0) by nia.
+      assert (- vx * (dx * uy - dy * ux) <= 0) by nia.
+      nia.
+    - assert (ux = 0) by nia.
+      subst ux.
+      destruct Hat as [Hat | [Hatx Haty]]; [nia |].
+      destruct Htq as [Htq | [Htqx Htqy]]; subst; nia.
+  }
+  subst dx dy ux uy vx vy.
+  ring_simplify in Hgoal_shift.
+  nia.
+Qed.
+
+Lemma left_equal_pop_support_upper :
+  forall q s t a,
+  leftdown t q ->
+  leftdown q s ->
+  leftdown t s ->
+  leftdown a t ->
+  ~ ccw s t a ->
+  Record_Geo_Vec.left_equal (build_vec t s) (build_vec t q) ->
+  Record_Geo_Vec.left_equal (build_vec a s) (build_vec a q).
+Proof.
+  unfold leftdown, ccw, Record_Geo_Vec.left_than,
+         Record_Geo_Vec.left_equal, Record_Geo_Vec.cross_prod, build_vec,
+         x, y.
+  simpl.
+  intros [qx qy] [sx sy] [tx ty] [ax ay] Htq Hqs Hts Hat Hturn Hedge.
+  simpl in *.
+  set (dx := sx - tx) in *.
+  set (dy := sy - ty) in *.
+  set (ux := tx - ax) in *.
+  set (uy := ty - ay) in *.
+  set (vx := qx - tx) in *.
+  set (vy := qy - ty) in *.
+  assert (Hturn' : dx * uy - dy * ux <= 0) by (subst; ring_simplify; nia).
+  assert (Hedge' : dx * vy - dy * vx <= 0) by (subst; ring_simplify; nia).
+  assert (Hdx : dx >= 0).
+  {
+    destruct Hts as [Hts | [Htsx Htsy]]; subst; nia.
+  }
+  assert (Hux_nonneg : 0 <= ux).
+  {
+    destruct Hat as [Hat | [Hatx Haty]]; subst; nia.
+  }
+  assert (Hvx_nonneg : 0 <= vx).
+  {
+    destruct Htq as [Htq | [Htqx Htqy]]; subst; nia.
+  }
+  assert (Hsv_nonneg : vx <= dx).
+  {
+    destruct Hqs as [Hqs | [Hqsx Hqsy]]; subst; nia.
+  }
+  assert (Hgoal_shift :
+    (ux + dx) * (vy + uy) - (uy + dy) * (vx + ux) <= 0).
+  {
+    assert (Hid :
+      dx * ((ux + dx) * (vy + uy) - (uy + dy) * (vx + ux)) =
+      (ux + dx) * (dx * vy - dy * vx) +
+      (dx - vx) * (dx * uy - dy * ux)) by ring.
+    destruct (Z.eq_dec dx 0) as [Hdx0 | Hdx_ne].
+    - subst dx.
+      assert (vx = 0) by nia.
+      subst vx.
+      nia.
+    - assert (Hdx_pos : dx > 0) by nia.
+      assert ((ux + dx) * (dx * vy - dy * vx) <= 0) by nia.
+      assert ((dx - vx) * (dx * uy - dy * ux) <= 0) by nia.
+      nia.
+  }
+  subst dx dy ux uy vx vy.
+  ring_simplify in Hgoal_shift.
+  nia.
+Qed.
+
+Lemma point_left_of_path_edges_push_support_lower :
+  forall q a t s rest,
+  leftdown s t ->
+  leftdown q t ->
+  leftdown t a ->
+  ccw s t a ->
+  point_left_of_path_edges q (t :: s :: rest) ->
+  point_left_of_path_edges q (a :: t :: s :: rest).
+Proof.
+  intros q a t s rest Hst Hqt Hta Hturn Hpath.
+  pose proof Hpath as Hpath_edge.
+  simpl in Hpath_edge.
+  destruct Hpath_edge as [Hedge _].
+  simpl.
+  split.
+  - exact (left_equal_push_support_lower
+             q s t a Hst Hqt Hta Hturn Hedge).
+  - exact Hpath.
+Qed.
+
+Lemma point_left_of_path_edges_pop_interval_lower :
+  forall q a t s rest,
+  leftdown s q ->
+  leftdown q t ->
+  leftdown s t ->
+  leftdown t a ->
+  ~ ccw s t a ->
+  point_left_of_path_edges q (t :: s :: rest) ->
+  point_left_of_path_edges q (a :: s :: rest).
+Proof.
+  intros q a t s rest Hsq Hqt Hst Hta Hturn Hpath.
+  simpl in Hpath |- *.
+  destruct Hpath as [Hedge Htail].
+  split.
+  - exact (left_equal_pop_support_lower
+             q s t a Hsq Hqt Hst Hta Hturn Hedge).
+  - exact Htail.
+Qed.
+
+Lemma point_left_of_path_edges_push_support_upper :
+  forall q a t s rest,
+  leftdown t s ->
+  leftdown t q ->
+  leftdown a t ->
+  ccw s t a ->
+  point_left_of_path_edges q (t :: s :: rest) ->
+  point_left_of_path_edges q (a :: t :: s :: rest).
+Proof.
+  intros q a t s rest Hts Htq Hat Hturn Hpath.
+  pose proof Hpath as Hpath_edge.
+  simpl in Hpath_edge.
+  destruct Hpath_edge as [Hedge _].
+  simpl.
+  split.
+  - exact (left_equal_push_support_upper
+             q s t a Hts Htq Hat Hturn Hedge).
+  - exact Hpath.
+Qed.
+
+Lemma point_left_of_path_edges_pop_interval_upper :
+  forall q a t s rest,
+  leftdown t q ->
+  leftdown q s ->
+  leftdown t s ->
+  leftdown a t ->
+  ~ ccw s t a ->
+  point_left_of_path_edges q (t :: s :: rest) ->
+  point_left_of_path_edges q (a :: s :: rest).
+Proof.
+  intros q a t s rest Htq Hqs Hts Hat Hturn Hpath.
+  simpl in Hpath |- *.
+  destruct Hpath as [Hedge Htail].
+  split.
+  - exact (left_equal_pop_support_upper
+             q s t a Htq Hqs Hts Hat Hturn Hedge).
+  - exact Htail.
+Qed.
+
+Lemma leftdown_total : forall p q,
+  leftdown p q \/ leftdown q p.
+Proof.
+  unfold leftdown, x, y.
+  intros [px py] [qx qy].
+  simpl; lia.
+Qed.
+
+Lemma point_xy_sorted_rev_stack_adjacent :
+  forall top s rest first,
+  point_xy_sorted (rev (top :: s :: rest ++ [first])) ->
+  leftdown s top.
+Proof.
+  intros top s rest first Hsorted.
+  simpl in Hsorted.
+  rewrite rev_app_distr in Hsorted.
+  simpl in Hsorted.
+  change (point_xy_sorted (first :: (rev rest ++ [s]) ++ [top]))
+    in Hsorted.
+  pose proof (point_xy_sorted_all_leftdown_last
+                first (rev rest ++ [s]) top Hsorted) as Hall.
+  rewrite Forall_forall in Hall.
+  apply Hall.
+  simpl.
+  right.
+  rewrite in_app_iff.
+  left.
+  rewrite in_app_iff.
+  right; simpl; auto.
+Qed.
+
+Lemma point_left_of_path_edges_graham_scan_inc_lower_between :
+  forall q a first top stack,
+  point_xy_sorted (rev (top :: stack ++ [first])) ->
+  Forall (fun r => leftdown r a) (top :: stack ++ [first]) ->
+  leftdown first q ->
+  leftdown q top ->
+  point_left_of_path_edges q (top :: stack ++ [first]) ->
+  point_left_of_path_edges q (graham_scan_inc a (top :: stack ++ [first])).
+Proof.
+  intros q a first top stack.
+  revert q a top.
+  induction stack as [| s rest IH]; intros q a top
+    Hsorted Hall Hfirstq Hqtop Hpath.
+  - change (top :: [] ++ [first]) with ([top; first])
+      in Hsorted, Hall, Hpath |- *.
+    simpl in Hall.
+    rewrite Forall_cons_iff in Hall.
+    destruct Hall as [Htopa Hall].
+    rewrite Forall_cons_iff in Hall.
+    destruct Hall as [Hfirsta _].
+    simpl in Hpath.
+    destruct (ccw_dec first top a) as [Hturn | Hnot] eqn:Hturn_dec.
+    + simpl.
+      rewrite Hturn_dec.
+      apply point_left_of_path_edges_push_support_lower.
+      * eapply leftdown_trans; eauto.
+      * exact Hqtop.
+      * exact Htopa.
+      * exact Hturn.
+      * exact Hpath.
+    + simpl.
+      rewrite Hturn_dec.
+      split.
+      * eapply left_equal_pop_support_lower.
+        -- exact Hfirstq.
+        -- exact Hqtop.
+        -- eapply leftdown_trans; eauto.
+        -- exact Htopa.
+        -- exact Hnot.
+        -- exact (proj1 Hpath).
+      * exact I.
+  - rewrite Forall_cons_iff in Hall.
+    destruct Hall as [Htopa Hall_tail].
+    pose proof (point_xy_sorted_rev_stack_adjacent
+                  top s rest first Hsorted) as Hstop.
+    destruct (ccw_dec s top a) as [Hturn | Hnot] eqn:Hturn_dec.
+    + simpl.
+      rewrite Hturn_dec.
+      apply point_left_of_path_edges_push_support_lower.
+      * exact Hstop.
+      * exact Hqtop.
+      * exact Htopa.
+      * exact Hturn.
+      * exact Hpath.
+    + destruct (leftdown_total s q) as [Hsq | Hqs].
+      * simpl.
+        rewrite Hturn_dec.
+        change (point_left_of_path_edges q
+          (graham_scan_inc a (s :: rest ++ [first]))).
+        apply point_left_of_path_edges_graham_scan_inc_cleanup.
+        eapply point_left_of_path_edges_pop_interval_lower.
+        -- exact Hsq.
+        -- exact Hqtop.
+        -- exact Hstop.
+        -- exact Htopa.
+        -- exact Hnot.
+        -- exact Hpath.
+      * simpl.
+        rewrite Hturn_dec.
+        change (point_left_of_path_edges q
+          (graham_scan_inc a (s :: rest ++ [first]))).
+        apply IH.
+        -- change (point_xy_sorted (rev (s :: rest ++ [first]))).
+           eapply point_xy_sorted_rev_tail.
+           exact Hsorted.
+        -- exact Hall_tail.
+        -- exact Hfirstq.
+        -- exact Hqs.
+        -- eapply point_left_of_path_edges_tail.
+           exact Hpath.
+Qed.
+
+Lemma point_xy_sorted_stack_adjacent :
+  forall top s rest last,
+  point_xy_sorted (top :: s :: rest ++ [last]) ->
+  leftdown top s.
+Proof.
+  intros top s rest last Hsorted.
+  simpl in Hsorted.
+  exact (proj1 Hsorted).
+Qed.
+
+Lemma point_left_of_path_edges_graham_scan_inc_upper_between :
+  forall q a last top stack,
+  point_xy_sorted (top :: stack ++ [last]) ->
+  Forall (fun r => leftdown a r) (top :: stack ++ [last]) ->
+  leftdown top q ->
+  leftdown q last ->
+  point_left_of_path_edges q (top :: stack ++ [last]) ->
+  point_left_of_path_edges q (graham_scan_inc a (top :: stack ++ [last])).
+Proof.
+  intros q a last top stack.
+  revert q a top.
+  induction stack as [| s rest IH]; intros q a top
+    Hsorted Hall Htopq Hqlast Hpath.
+  - change (top :: [] ++ [last]) with ([top; last])
+      in Hsorted, Hall, Hpath |- *.
+    simpl in Hall.
+    rewrite Forall_cons_iff in Hall.
+    destruct Hall as [Hatop Hall].
+    rewrite Forall_cons_iff in Hall.
+    destruct Hall as [Halast _].
+    simpl in Hpath.
+    destruct (ccw_dec last top a) as [Hturn | Hnot] eqn:Hturn_dec.
+    + simpl.
+      rewrite Hturn_dec.
+      apply point_left_of_path_edges_push_support_upper.
+      * eapply leftdown_trans; eauto.
+      * exact Htopq.
+      * exact Hatop.
+      * exact Hturn.
+      * exact Hpath.
+    + simpl.
+      rewrite Hturn_dec.
+      split.
+      * eapply left_equal_pop_support_upper.
+        -- exact Htopq.
+        -- exact Hqlast.
+        -- eapply leftdown_trans; eauto.
+        -- exact Hatop.
+        -- exact Hnot.
+        -- exact (proj1 Hpath).
+      * exact I.
+  - rewrite Forall_cons_iff in Hall.
+    destruct Hall as [Hatop Hall_tail].
+    pose proof (point_xy_sorted_stack_adjacent
+                  top s rest last Hsorted) as Htops.
+    destruct (ccw_dec s top a) as [Hturn | Hnot] eqn:Hturn_dec.
+    + simpl.
+      rewrite Hturn_dec.
+      apply point_left_of_path_edges_push_support_upper.
+      * exact Htops.
+      * exact Htopq.
+      * exact Hatop.
+      * exact Hturn.
+      * exact Hpath.
+    + destruct (leftdown_total q s) as [Hqs | Hsq].
+      * simpl.
+        rewrite Hturn_dec.
+        change (point_left_of_path_edges q
+          (graham_scan_inc a (s :: rest ++ [last]))).
+        apply point_left_of_path_edges_graham_scan_inc_cleanup.
+        eapply point_left_of_path_edges_pop_interval_upper.
+        -- exact Htopq.
+        -- exact Hqs.
+        -- exact Htops.
+        -- exact Hatop.
+        -- exact Hnot.
+        -- exact Hpath.
+      * simpl.
+        rewrite Hturn_dec.
+        change (point_left_of_path_edges q
+          (graham_scan_inc a (s :: rest ++ [last]))).
+        apply IH.
+        -- eapply point_xy_sorted_tail.
+           exact Hsorted.
+        -- exact Hall_tail.
+        -- exact Hsq.
+        -- exact Hqlast.
+        -- eapply point_left_of_path_edges_tail.
+           exact Hpath.
+Qed.
+
+Lemma left_equal_to_endpoint : forall p q,
+  Record_Geo_Vec.left_equal (build_vec p q) (build_vec p p).
+Proof.
+  unfold Record_Geo_Vec.left_equal, Record_Geo_Vec.cross_prod, build_vec.
+  simpl; intros; nia.
+Qed.
+
+Lemma left_equal_to_edge_endpoint : forall p q,
+  Record_Geo_Vec.left_equal (build_vec p q) (build_vec p q).
+Proof.
+  unfold Record_Geo_Vec.left_equal.
+  intros; rewrite Record_Geo_Vec.cross_prod_self; lia.
+Qed.
+
+Lemma ccw_rev_edge_left_equal : forall p q r,
+  ccw p q r ->
+  Record_Geo_Vec.left_equal (build_vec q p) (build_vec q r).
+Proof.
+  unfold ccw, Record_Geo_Vec.left_than, Record_Geo_Vec.left_equal,
+         Record_Geo_Vec.cross_prod, build_vec.
+  simpl; intros; nia.
+Qed.
+
+Lemma point_xy_sorted_rev_stack_all_leftdown_head :
+  forall top stack first,
+  point_xy_sorted (rev (top :: stack ++ [first])) ->
+  Forall (fun r => leftdown r top) (top :: stack ++ [first]).
+Proof.
+  intros top stack first Hsorted.
+  assert (Hsorted' : point_xy_sorted (first :: rev stack ++ [top])).
+  {
+    simpl in Hsorted.
+    rewrite rev_app_distr in Hsorted.
+    simpl in Hsorted.
+    exact Hsorted.
+  }
+  pose proof (point_xy_sorted_all_leftdown_last
+                first (rev stack) top Hsorted') as Hall.
+  replace (top :: stack ++ [first])
+    with (rev (first :: rev stack ++ [top])).
+  - apply Forall_rev.
+    exact Hall.
+  - simpl.
+    rewrite rev_app_distr.
+    simpl.
+    rewrite rev_involutive.
+    reflexivity.
+Qed.
+
+Lemma point_xy_sorted_stack_all_leftdown_head :
+  forall top stack last,
+  point_xy_sorted (top :: stack ++ [last]) ->
+  Forall (fun r => leftdown top r) (top :: stack ++ [last]).
+Proof.
+  intros top stack last Hsorted.
+  constructor.
+  - apply leftdown_refl.
+  - simpl in Hsorted.
+    apply point_xy_sorted_from_leftdown_head.
+    exact Hsorted.
+Qed.
+
+Lemma point_left_of_path_edges_lower_after_turn :
+  forall a first top s rest,
+  point_xy_sorted (rev (top :: s :: rest ++ [first])) ->
+  rev_consec_ccw (top :: s :: rest ++ [first]) ->
+  Forall (fun r => leftdown r a) (top :: s :: rest ++ [first]) ->
+  ccw s top a ->
+  point_left_of_path_edges a (top :: s :: rest ++ [first]).
+Proof.
+  intros a first top s rest.
+  revert a first top s.
+  induction rest as [| u rest IH]; intros a first top s
+    Hsorted Hcon Hall Hturn.
+  - assert (Hfirsts : leftdown first s).
+    {
+      simpl in Hsorted.
+      destruct Hsorted as [Hfirsts _].
+      exact Hfirsts.
+    }
+    assert (Hstop : leftdown s top).
+    {
+      simpl in Hsorted.
+      destruct Hsorted as [_ [Hstop _]].
+      exact Hstop.
+    }
+    assert (Htopa : leftdown top a).
+    {
+      rewrite Forall_cons_iff in Hall.
+      exact (proj1 Hall).
+    }
+    assert (Hfirst_s_top : ccw first s top).
+    {
+      simpl in Hcon.
+      destruct Hcon as [Hs_top_first _].
+      apply ccw_cyclicity_2.
+      exact Hs_top_first.
+    }
+    assert (Hfirst_s_a : ccw first s a).
+    {
+      eapply ccw_leftdown_forward_extend_head; eauto.
+    }
+    simpl.
+    split.
+    + apply ccw_rev_edge_left_equal.
+      exact Hturn.
+    + split.
+      * apply ccw_rev_edge_left_equal.
+        exact Hfirst_s_a.
+      * exact I.
+  - assert (Htail_sorted :
+      point_xy_sorted (rev (s :: u :: rest ++ [first]))).
+    {
+      change (point_xy_sorted (rev (s :: u :: rest ++ [first]))).
+      eapply point_xy_sorted_rev_tail.
+      exact Hsorted.
+    }
+    assert (Hstop : leftdown s top).
+    {
+      eapply point_xy_sorted_rev_stack_adjacent.
+      exact Hsorted.
+    }
+    assert (Hus : leftdown u s).
+    {
+      eapply point_xy_sorted_rev_stack_adjacent.
+      exact Htail_sorted.
+    }
+    assert (Htopa : leftdown top a).
+    {
+      rewrite Forall_cons_iff in Hall.
+      exact (proj1 Hall).
+    }
+    assert (Htail_con : rev_consec_ccw (s :: u :: rest ++ [first])).
+    {
+      apply rev_consec_ccw_cons_iff in Hcon as [Htail _].
+      exact Htail.
+    }
+    assert (Hu_s_top : ccw u s top).
+    {
+      apply rev_consec_ccw_cons_iff in Hcon as [_ Hhead].
+      apply ccw_cyclicity_2.
+      apply (Hhead s u (rest ++ [first])).
+      reflexivity.
+    }
+    assert (Hu_s_a : ccw u s a).
+    {
+      eapply ccw_leftdown_forward_extend_head; eauto.
+    }
+    rewrite Forall_cons_iff in Hall.
+    destruct Hall as [_ Hall_tail].
+    simpl.
+    split.
+    + apply ccw_rev_edge_left_equal.
+      exact Hturn.
+    + eapply IH; eauto.
+Qed.
+
+Lemma point_left_of_path_edges_upper_after_turn :
+  forall a last top s rest,
+  point_xy_sorted (top :: s :: rest ++ [last]) ->
+  rev_consec_ccw (top :: s :: rest ++ [last]) ->
+  Forall (fun r => leftdown a r) (top :: s :: rest ++ [last]) ->
+  ccw s top a ->
+  point_left_of_path_edges a (top :: s :: rest ++ [last]).
+Proof.
+  intros a last top s rest.
+  revert a last top s.
+  induction rest as [| u rest IH]; intros a last top s
+    Hsorted Hcon Hall Hturn.
+  - assert (Htops : leftdown top s).
+    {
+      simpl in Hsorted.
+      exact (proj1 Hsorted).
+    }
+    assert (Hslast : leftdown s last).
+    {
+      simpl in Hsorted.
+      destruct Hsorted as [_ [Hslast _]].
+      exact Hslast.
+    }
+    assert (Hatop : leftdown a top).
+    {
+      rewrite Forall_cons_iff in Hall.
+      exact (proj1 Hall).
+    }
+    assert (Hlast_s_top : ccw last s top).
+    {
+      simpl in Hcon.
+      destruct Hcon as [Hs_top_last _].
+      apply ccw_cyclicity_2.
+      exact Hs_top_last.
+    }
+    assert (Hlast_s_a : ccw last s a).
+    {
+      eapply ccw_leftdown_rev_forward_extend_head; eauto.
+    }
+    simpl.
+    split.
+    + apply ccw_rev_edge_left_equal.
+      exact Hturn.
+    + split.
+      * apply ccw_rev_edge_left_equal.
+        exact Hlast_s_a.
+      * exact I.
+  - assert (Htail_sorted :
+      point_xy_sorted (s :: u :: rest ++ [last])).
+    {
+      eapply point_xy_sorted_tail.
+      exact Hsorted.
+    }
+    assert (Htops : leftdown top s).
+    {
+      eapply point_xy_sorted_stack_adjacent.
+      exact Hsorted.
+    }
+    assert (Hsu : leftdown s u).
+    {
+      eapply point_xy_sorted_stack_adjacent.
+      exact Htail_sorted.
+    }
+    assert (Hatop : leftdown a top).
+    {
+      rewrite Forall_cons_iff in Hall.
+      exact (proj1 Hall).
+    }
+    assert (Htail_con : rev_consec_ccw (s :: u :: rest ++ [last])).
+    {
+      apply rev_consec_ccw_cons_iff in Hcon as [Htail _].
+      exact Htail.
+    }
+    assert (Hu_s_top : ccw u s top).
+    {
+      apply rev_consec_ccw_cons_iff in Hcon as [_ Hhead].
+      apply ccw_cyclicity_2.
+      apply (Hhead s u (rest ++ [last])).
+      reflexivity.
+    }
+    assert (Hu_s_a : ccw u s a).
+    {
+      eapply ccw_leftdown_rev_forward_extend_head; eauto.
+    }
+    rewrite Forall_cons_iff in Hall.
+    destruct Hall as [_ Hall_tail].
+    simpl.
+    split.
+    + apply ccw_rev_edge_left_equal.
+      exact Hturn.
+    + eapply IH; eauto.
+Qed.
+
+Lemma point_left_of_path_edges_graham_scan_inc_lower_self :
+  forall a first top stack,
+  point_xy_sorted (rev (top :: stack ++ [first])) ->
+  rev_consec_ccw (top :: stack ++ [first]) ->
+  Forall (fun r => leftdown r a) (top :: stack ++ [first]) ->
+  point_left_of_path_edges a (graham_scan_inc a (top :: stack ++ [first])).
+Proof.
+  intros a first top stack.
+  revert a first top.
+  induction stack as [| s rest IH]; intros a first top
+    Hsorted Hcon Hall.
+  - change (top :: [] ++ [first]) with ([top; first])
+      in Hsorted, Hcon, Hall |- *.
+    simpl.
+    destruct (ccw_dec first top a) as [Hturn | _].
+    + simpl.
+      split.
+      * apply left_equal_to_endpoint.
+      * split.
+        -- apply ccw_rev_edge_left_equal.
+           exact Hturn.
+        -- exact I.
+    + simpl.
+      split; [apply left_equal_to_endpoint | exact I].
+  - pose proof Hall as Hall_all.
+    rewrite Forall_cons_iff in Hall.
+    destruct Hall as [_ Hall_tail].
+    simpl.
+    destruct (ccw_dec s top a) as [Hturn | _].
+    + simpl.
+      split.
+      * apply left_equal_to_endpoint.
+      * eapply point_left_of_path_edges_lower_after_turn; eauto.
+    + change (point_left_of_path_edges a
+        (graham_scan_inc a (s :: rest ++ [first]))).
+      apply IH.
+      * change (point_xy_sorted (rev (s :: rest ++ [first]))).
+        eapply point_xy_sorted_rev_tail.
+        exact Hsorted.
+      * apply rev_consec_ccw_cons_iff in Hcon as [Htail _].
+        exact Htail.
+      * exact Hall_tail.
+Qed.
+
+Lemma point_left_of_path_edges_graham_scan_inc_upper_self :
+  forall a last top stack,
+  point_xy_sorted (top :: stack ++ [last]) ->
+  rev_consec_ccw (top :: stack ++ [last]) ->
+  Forall (fun r => leftdown a r) (top :: stack ++ [last]) ->
+  point_left_of_path_edges a (graham_scan_inc a (top :: stack ++ [last])).
+Proof.
+  intros a last top stack.
+  revert a last top.
+  induction stack as [| s rest IH]; intros a last top
+    Hsorted Hcon Hall.
+  - change (top :: [] ++ [last]) with ([top; last])
+      in Hsorted, Hcon, Hall |- *.
+    simpl.
+    destruct (ccw_dec last top a) as [Hturn | _].
+    + simpl.
+      split.
+      * apply left_equal_to_endpoint.
+      * split.
+        -- apply ccw_rev_edge_left_equal.
+           exact Hturn.
+        -- exact I.
+    + simpl.
+      split; [apply left_equal_to_endpoint | exact I].
+  - pose proof Hall as Hall_all.
+    rewrite Forall_cons_iff in Hall.
+    destruct Hall as [_ Hall_tail].
+    simpl.
+    destruct (ccw_dec s top a) as [Hturn | _].
+    + simpl.
+      split.
+      * apply left_equal_to_endpoint.
+      * eapply point_left_of_path_edges_upper_after_turn; eauto.
+    + change (point_left_of_path_edges a
+        (graham_scan_inc a (s :: rest ++ [last]))).
+      apply IH.
+      * eapply point_xy_sorted_tail.
+        exact Hsorted.
+      * apply rev_consec_ccw_cons_iff in Hcon as [Htail _].
+        exact Htail.
+      * exact Hall_tail.
+Qed.
+
+Lemma graham_scan_inc_preserves_stack_sorted_upper : forall p T,
+  Forall (fun q => leftdown p q) T ->
+  point_xy_sorted T ->
+  point_xy_sorted (graham_scan_inc p T).
+Proof.
+  intros p T Hall Hsorted.
+  replace (graham_scan_inc p T)
+    with (rev (rev (graham_scan_inc p T)))
+    by apply rev_involutive.
+  apply point_xy_rev_sorted_rev_is_sorted.
+  apply graham_scan_inc_preserves_rev_sorted_chain.
+  - exact Hall.
+  - apply point_xy_sorted_rev_is_rev_sorted.
+    exact Hsorted.
+Qed.
+
+Lemma fold_left_graham_scan_inc_lower_open_edges_aux :
+  forall first top stack rest L,
+  point_xy_sorted (rev (top :: stack ++ [first])) ->
+  rev_consec_ccw (top :: stack ++ [first]) ->
+  point_xy_sorted_from top rest ->
+  Forall (fun q => leftdown first q) L ->
+  Forall (fun q => leftdown q top) L ->
+  Forall
+    (fun q => point_left_of_path_edges q (top :: stack ++ [first]))
+    L ->
+  Forall
+    (fun q =>
+       point_left_of_path_edges q
+         (fold_left (fun T p => graham_scan_inc p T)
+            rest (top :: stack ++ [first])))
+    (L ++ rest).
+Proof.
+  intros first top stack rest.
+  revert first top stack.
+  induction rest as [| a rest IH]; intros first top stack L
+    Hsorted Hcon Hrest Hfirst_L Htop_L Hcover_L.
+  - simpl.
+    rewrite app_nil_r.
+    exact Hcover_L.
+  - simpl in Hrest.
+    destruct Hrest as [Htopa Hrest].
+    assert (Hall : Forall (fun r => leftdown r a)
+      (top :: stack ++ [first])).
+    {
+      eapply Forall_impl.
+      - intros r Hrtop.
+        eapply leftdown_trans.
+        + exact Hrtop.
+        + exact Htopa.
+      - apply point_xy_sorted_rev_stack_all_leftdown_head.
+        exact Hsorted.
+    }
+    assert (Hcover_old :
+      Forall
+        (fun q =>
+           point_left_of_path_edges q
+             (graham_scan_inc a (top :: stack ++ [first])))
+        L).
+    {
+      rewrite Forall_forall.
+      intros q Hq.
+      eapply point_left_of_path_edges_graham_scan_inc_lower_between.
+      - exact Hsorted.
+      - exact Hall.
+      - rewrite Forall_forall in Hfirst_L.
+        exact (Hfirst_L q Hq).
+      - rewrite Forall_forall in Htop_L.
+        exact (Htop_L q Hq).
+      - rewrite Forall_forall in Hcover_L.
+        exact (Hcover_L q Hq).
+    }
+    assert (Hcover_a :
+      point_left_of_path_edges a
+        (graham_scan_inc a (top :: stack ++ [first]))).
+    {
+      eapply point_left_of_path_edges_graham_scan_inc_lower_self; eauto.
+    }
+    assert (Hfirsta : leftdown first a).
+    {
+      rewrite Forall_forall in Hall.
+      apply Hall.
+      simpl.
+      right.
+      rewrite in_app_iff.
+      right.
+      simpl; auto.
+    }
+    destruct (graham_scan_inc_preserves_bottom_with_head
+                a (top :: stack) first) as [stack' Hshape].
+    change (graham_scan_inc a (top :: stack ++ [first]) =
+              a :: stack' ++ [first]) in Hshape.
+    change (fold_left (fun T p => graham_scan_inc p T)
+              (a :: rest) (top :: stack ++ [first]))
+      with (fold_left (fun T p => graham_scan_inc p T)
+              rest (graham_scan_inc a (top :: stack ++ [first]))).
+    rewrite Hshape.
+    replace (L ++ a :: rest) with ((L ++ [a]) ++ rest)
+      by (rewrite <- app_assoc; reflexivity).
+    apply IH.
+    + rewrite <- Hshape.
+      apply graham_scan_inc_preserves_sorted_chain; assumption.
+    + rewrite <- Hshape.
+      apply graham_scan_inc_rev_consec.
+      exact Hcon.
+    + exact Hrest.
+    + rewrite Forall_app.
+      split.
+      * exact Hfirst_L.
+      * constructor; [exact Hfirsta | constructor].
+    + rewrite Forall_app.
+      split.
+      * eapply Forall_impl.
+        -- intros q Hqtop.
+           eapply leftdown_trans.
+           ++ exact Hqtop.
+           ++ exact Htopa.
+        -- exact Htop_L.
+      * constructor; [apply leftdown_refl | constructor].
+    + rewrite Forall_app.
+      split.
+      * rewrite <- Hshape.
+        exact Hcover_old.
+      * constructor.
+        -- rewrite <- Hshape.
+           exact Hcover_a.
+        -- constructor.
+Qed.
+
+Lemma fold_left_graham_scan_inc_upper_open_edges_aux :
+  forall last top stack rest L,
+  point_xy_sorted (top :: stack ++ [last]) ->
+  rev_consec_ccw (top :: stack ++ [last]) ->
+  point_xy_rev_sorted_from top rest ->
+  Forall (fun q => leftdown top q) L ->
+  Forall (fun q => leftdown q last) L ->
+  Forall
+    (fun q => point_left_of_path_edges q (top :: stack ++ [last]))
+    L ->
+  Forall
+    (fun q =>
+       point_left_of_path_edges q
+         (fold_left (fun T p => graham_scan_inc p T)
+            rest (top :: stack ++ [last])))
+    (L ++ rest).
+Proof.
+  intros last top stack rest.
+  revert last top stack.
+  induction rest as [| a rest IH]; intros last top stack L
+    Hsorted Hcon Hrest Htop_L Hlast_L Hcover_L.
+  - simpl.
+    rewrite app_nil_r.
+    exact Hcover_L.
+  - simpl in Hrest.
+    destruct Hrest as [Hatop Hrest].
+    assert (Hall : Forall (fun r => leftdown a r)
+      (top :: stack ++ [last])).
+    {
+      eapply Forall_impl.
+      - intros r Htopr.
+        eapply leftdown_trans.
+        + exact Hatop.
+        + exact Htopr.
+      - apply point_xy_sorted_stack_all_leftdown_head.
+        exact Hsorted.
+    }
+    assert (Hcover_old :
+      Forall
+        (fun q =>
+           point_left_of_path_edges q
+             (graham_scan_inc a (top :: stack ++ [last])))
+        L).
+    {
+      rewrite Forall_forall.
+      intros q Hq.
+      eapply point_left_of_path_edges_graham_scan_inc_upper_between.
+      - exact Hsorted.
+      - exact Hall.
+      - rewrite Forall_forall in Htop_L.
+        exact (Htop_L q Hq).
+      - rewrite Forall_forall in Hlast_L.
+        exact (Hlast_L q Hq).
+      - rewrite Forall_forall in Hcover_L.
+        exact (Hcover_L q Hq).
+    }
+    assert (Hcover_a :
+      point_left_of_path_edges a
+        (graham_scan_inc a (top :: stack ++ [last]))).
+    {
+      eapply point_left_of_path_edges_graham_scan_inc_upper_self; eauto.
+    }
+    assert (Halast : leftdown a last).
+    {
+      rewrite Forall_forall in Hall.
+      apply Hall.
+      simpl.
+      right.
+      rewrite in_app_iff.
+      right.
+      simpl; auto.
+    }
+    destruct (graham_scan_inc_preserves_bottom_with_head
+                a (top :: stack) last) as [stack' Hshape].
+    change (graham_scan_inc a (top :: stack ++ [last]) =
+              a :: stack' ++ [last]) in Hshape.
+    change (fold_left (fun T p => graham_scan_inc p T)
+              (a :: rest) (top :: stack ++ [last]))
+      with (fold_left (fun T p => graham_scan_inc p T)
+              rest (graham_scan_inc a (top :: stack ++ [last]))).
+    rewrite Hshape.
+    replace (L ++ a :: rest) with ((L ++ [a]) ++ rest)
+      by (rewrite <- app_assoc; reflexivity).
+    apply IH.
+    + rewrite <- Hshape.
+      apply graham_scan_inc_preserves_stack_sorted_upper; assumption.
+    + rewrite <- Hshape.
+      apply graham_scan_inc_rev_consec.
+      exact Hcon.
+    + exact Hrest.
+    + rewrite Forall_app.
+      split.
+      * eapply Forall_impl.
+        -- intros q Htopq.
+           eapply leftdown_trans.
+           ++ exact Hatop.
+           ++ exact Htopq.
+        -- exact Htop_L.
+      * constructor; [apply leftdown_refl | constructor].
+    + rewrite Forall_app.
+      split.
+      * exact Hlast_L.
+      * constructor; [exact Halast | constructor].
+    + rewrite Forall_app.
+      split.
+      * rewrite <- Hshape.
+        exact Hcover_old.
+      * constructor.
+        -- rewrite <- Hshape.
+           exact Hcover_a.
+        -- constructor.
+Qed.
+
+Lemma fold_left_graham_scan_inc_lower_open_edges :
+  forall first second rest,
+  point_xy_sorted (first :: second :: rest) ->
+  Forall
+    (fun q =>
+       point_left_of_path_edges q
+         (andrew_scan_stack (first :: second :: rest)))
+    (first :: second :: rest).
+Proof.
+  intros first second rest Hsorted.
+  simpl in Hsorted.
+  destruct Hsorted as [Hfirst_second Hsorted_rest].
+  unfold andrew_scan_stack.
+  simpl.
+  eapply (fold_left_graham_scan_inc_lower_open_edges_aux
+            first second [] rest [first; second]).
+  - simpl.
+    split; [exact Hfirst_second | exact I].
+  - simpl; repeat split.
+  - exact Hsorted_rest.
+  - constructor; [apply leftdown_refl |].
+    constructor; [exact Hfirst_second | constructor].
+  - constructor; [exact Hfirst_second |].
+    constructor; [apply leftdown_refl | constructor].
+  - rewrite !Forall_cons_iff.
+    split.
+    + simpl.
+      split; [apply left_equal_to_edge_endpoint | exact I].
+    + split.
+      * simpl.
+        split; [apply left_equal_to_endpoint | exact I].
+      * apply Forall_nil.
+Qed.
+
+Lemma fold_left_graham_scan_inc_upper_open_edges :
+  forall last second rest,
+  point_xy_rev_sorted (last :: second :: rest) ->
+  Forall
+    (fun q =>
+       point_left_of_path_edges q
+         (andrew_scan_stack (last :: second :: rest)))
+    (last :: second :: rest).
+Proof.
+  intros last second rest Hsorted.
+  simpl in Hsorted.
+  destruct Hsorted as [Hsecond_last Hsorted_rest].
+  unfold andrew_scan_stack.
+  simpl.
+  eapply (fold_left_graham_scan_inc_upper_open_edges_aux
+            last second [] rest [last; second]).
+  - simpl.
+    split; [exact Hsecond_last | exact I].
+  - simpl; repeat split.
+  - exact Hsorted_rest.
+  - constructor; [exact Hsecond_last |].
+    constructor; [apply leftdown_refl | constructor].
+  - constructor; [apply leftdown_refl |].
+    constructor; [exact Hsecond_last | constructor].
+  - rewrite !Forall_cons_iff.
+    split.
+    + simpl.
+      split; [apply left_equal_to_edge_endpoint | exact I].
+    + split.
+      * simpl.
+        split; [apply left_equal_to_endpoint | exact I].
+      * apply Forall_nil.
+Qed.
+
+Lemma andrew_lower_chain_open_edge_cover :
+  forall first middle last lower_mid,
+  point_xy_sorted (first :: middle ++ [last]) ->
+  andrew_lower_chain (first :: middle ++ [last]) =
+    first :: lower_mid ++ [last] ->
+  Forall
+    (fun q =>
+       point_left_of_path_edges q (last :: rev lower_mid ++ [first]))
+    (first :: middle ++ [last]).
+Proof.
+  intros first middle last lower_mid Hsorted Hlower.
+  pose proof (andrew_lower_chain_stack_shape
+                first middle last lower_mid Hlower) as Hstack.
+  destruct middle as [| second middle].
+  - rewrite <- Hstack.
+    simpl.
+    rewrite !Forall_cons_iff.
+    split.
+    + simpl.
+      split; [apply left_equal_to_edge_endpoint | exact I].
+    + split.
+      * simpl.
+        split; [apply left_equal_to_endpoint | exact I].
+      * apply Forall_nil.
+  - pose proof (fold_left_graham_scan_inc_lower_open_edges
+                  first second (middle ++ [last]) Hsorted) as Hcover.
+    change (andrew_scan_stack (first :: second :: middle ++ [last]) =
+              last :: rev lower_mid ++ [first]) in Hstack.
+    rewrite Hstack in Hcover.
+    exact Hcover.
+Qed.
+
+Lemma andrew_upper_chain_open_edge_cover :
+  forall first middle last upper_mid,
+  point_xy_sorted (first :: middle ++ [last]) ->
+  andrew_upper_chain (first :: middle ++ [last]) =
+    last :: upper_mid ++ [first] ->
+  Forall
+    (fun q =>
+       point_left_of_path_edges q (first :: rev upper_mid ++ [last]))
+    (first :: middle ++ [last]).
+Proof.
+  intros first middle last upper_mid Hsorted Hupper.
+  pose proof (andrew_upper_chain_stack_shape
+                first middle last upper_mid Hupper) as Hstack.
+  assert (Hrev_sorted :
+    point_xy_rev_sorted (rev (first :: middle ++ [last]))).
+  {
+    apply point_xy_sorted_rev_is_rev_sorted.
+    exact Hsorted.
+  }
+  assert (Hcover_rev :
+    Forall
+      (fun q =>
+         point_left_of_path_edges q
+           (andrew_scan_stack (rev (first :: middle ++ [last]))))
+      (rev (first :: middle ++ [last]))).
+  {
+    replace (rev (first :: middle ++ [last]))
+      with (last :: rev middle ++ [first]) in Hrev_sorted |- *.
+    2: {
+      simpl.
+      rewrite rev_app_distr.
+      simpl.
+      reflexivity.
+    }
+    destruct (rev middle) as [| second rest].
+    - change (last :: [] ++ [first]) with ([last; first])
+        in Hrev_sorted |- *.
+      apply fold_left_graham_scan_inc_upper_open_edges.
+      exact Hrev_sorted.
+    - change (last :: (second :: rest) ++ [first]) with
+        (last :: second :: rest ++ [first]) in Hrev_sorted |- *.
+      apply fold_left_graham_scan_inc_upper_open_edges.
+      exact Hrev_sorted.
+  }
+  rewrite Hstack in Hcover_rev.
+  apply Forall_rev in Hcover_rev.
+  rewrite rev_involutive in Hcover_rev.
+  exact Hcover_rev.
+Qed.
+
+Lemma point_in_hull_edges_aux_from_path_edges :
+  forall q first prev rest,
+  point_left_of_path_edges q (prev :: rest ++ [first]) ->
+  point_in_hull_edges_aux_ q first prev rest.
+Proof.
+  intros q first prev rest.
+  revert prev.
+  induction rest as [| p rest IH]; intros prev Hpath.
+  - simpl in Hpath |- *.
+    tauto.
+  - simpl in Hpath |- *.
+    destruct Hpath as [Hedge Hpath].
+    split.
+    + apply IH.
+      exact Hpath.
+    + exact Hedge.
+Qed.
+
+Lemma point_in_hull_edges_from_closed_path_edges :
+  forall q first second third rest,
+  point_left_of_path_edges q (first :: second :: third :: rest ++ [first]) ->
+  point_in_hull_edges q (first :: second :: third :: rest).
+Proof.
+  intros q first second third rest Hpath.
+  simpl in Hpath |- *.
+  destruct Hpath as [Hedge Hpath].
+  split.
+  - exact Hedge.
+  - destruct Hpath as [Hedge' Hpath].
+    split.
+    + apply point_in_hull_edges_aux_from_path_edges.
+      exact Hpath.
+    + exact Hedge'.
+Qed.
+
+Lemma point_left_of_path_edges_from_aux :
+  forall q first prev rest,
+  point_in_hull_edges_aux_ q first prev rest ->
+  point_left_of_path_edges_from q prev (rest ++ [first]).
+Proof.
+  intros q first prev rest.
+  revert prev.
+  induction rest as [| p rest IH]; intros prev Haux.
+  - simpl in Haux |- *.
+    split; [exact Haux | exact I].
+  - simpl in Haux |- *.
+    destruct Haux as [Haux Hedge].
+    split.
+    + exact Hedge.
+    + apply IH.
+      exact Haux.
+Qed.
+
+Lemma point_left_of_path_edges_from_hull_edges :
+  forall q first second third rest,
+  point_in_hull_edges q (first :: second :: third :: rest) ->
+  point_left_of_path_edges q (first :: second :: third :: rest ++ [first]).
+Proof.
+  intros q first second third rest Hedges.
+  simpl in Hedges |- *.
+  destruct Hedges as [Hfirst Haux].
+  split.
+  - exact Hfirst.
+  - simpl in Haux.
+    destruct Haux as [Haux Hsecond].
+    split.
+    + exact Hsecond.
+    + apply point_left_of_path_edges_from_aux.
+      exact Haux.
+Qed.
+
+Lemma point_in_hull_edges_two_path_segment :
+  forall q first last,
+  Record_Geo_Vec.left_equal (build_vec first last) (build_vec first q) ->
+  Record_Geo_Vec.left_equal (build_vec last first) (build_vec last q) ->
+  leftdown first q ->
+  leftdown q last ->
+  point_in_hull_edges q [last; first].
+Proof.
+  intros q first last Hfl Hlf Hfirst Hlast.
+  simpl.
+  assert (Hcol : colinear q first last).
+  {
+    eapply opposite_left_equal_colinear; eauto.
+  }
+  split.
+  - apply colinear_comm.
+    exact Hcol.
+  - apply at_mid_comm.
+    apply leftdown_colinear_between_at_mid; assumption.
+Qed.
+
+Lemma point_left_of_path_edges_two_paths :
+  forall q first upper last lower final,
+  point_left_of_path_edges q (first :: upper ++ [last]) ->
+  point_left_of_path_edges q (last :: lower ++ [final]) ->
+  point_left_of_path_edges q ((first :: upper ++ last :: lower) ++ [final]).
+Proof.
+  intros q first upper.
+  revert first.
+  induction upper as [| u upper IH]; intros first last lower final Hupper Hlower.
+  - simpl in Hupper |- *.
+    destruct Hupper as [Hedge _].
+    split.
+    + exact Hedge.
+    + exact Hlower.
+  - simpl in Hupper |- *.
+    destruct Hupper as [Hedge Hupper].
+    split.
+    + exact Hedge.
+    + apply IH; assumption.
+Qed.
+
+Lemma point_in_hull_edges_from_two_open_paths :
+  forall q first upper last lower,
+  upper <> [] \/ lower <> [] ->
+  point_left_of_path_edges q (first :: upper ++ [last]) ->
+  point_left_of_path_edges q (last :: lower ++ [first]) ->
+  point_in_hull_edges q (first :: upper ++ last :: lower).
+Proof.
+  intros q first upper last lower Hnon Hupper Hlower.
+  pose proof (point_left_of_path_edges_two_paths
+                q first upper last lower first Hupper Hlower) as Hclosed.
+  destruct upper as [| u upper].
+  - destruct lower as [| l lower].
+    + destruct Hnon as [Hbad | Hbad]; contradiction Hbad; reflexivity.
+    + simpl in Hclosed |- *.
+      apply point_in_hull_edges_from_closed_path_edges.
+      exact Hclosed.
+  - simpl in Hclosed |- *.
+    destruct upper as [| u' upper].
+    + apply point_in_hull_edges_from_closed_path_edges.
+      exact Hclosed.
+    + apply point_in_hull_edges_from_closed_path_edges.
+      exact Hclosed.
+Qed.
+
+Lemma point_in_hull_edges_andrew_merge_from_two_paths :
+  forall q first lower_mid last upper_mid,
+  upper_mid <> [] \/ lower_mid <> [] ->
+  point_left_of_path_edges q (first :: rev upper_mid ++ [last]) ->
+  point_left_of_path_edges q (last :: rev lower_mid ++ [first]) ->
+  point_in_hull_edges q (rev upper_mid ++ last :: rev lower_mid ++ [first]).
+Proof.
+  intros q first lower_mid last upper_mid Hnon Hupper Hlower.
+  replace (rev upper_mid ++ last :: rev lower_mid ++ [first])
+    with ((rev upper_mid ++ last :: rev lower_mid) ++ [first])
+    by (rewrite <- app_assoc; reflexivity).
+  apply gs_point_in_hull_edges_rotate1.
+  change (first :: rev upper_mid ++ last :: rev lower_mid)
+    with (first :: rev upper_mid ++ last :: rev lower_mid).
+  apply point_in_hull_edges_from_two_open_paths.
+  - destruct Hnon as [Hupper_non | Hlower_non].
+    + left.
+      intro Hrev_nil.
+      apply Hupper_non.
+      apply (f_equal (@rev point)) in Hrev_nil.
+      rewrite rev_involutive in Hrev_nil.
+      exact Hrev_nil.
+    + right.
+      intro Hrev_nil.
+      apply Hlower_non.
+      apply (f_equal (@rev point)) in Hrev_nil.
+      rewrite rev_involutive in Hrev_nil.
+      exact Hrev_nil.
+  - exact Hupper.
+  - exact Hlower.
+Qed.
+
+Lemma andrew_hull_max_from_open_edge_covers :
+  forall first middle last lower_mid upper_mid,
+  point_xy_sorted (first :: middle ++ [last]) ->
+  andrew_lower_chain (first :: middle ++ [last]) =
+    first :: lower_mid ++ [last] ->
+  andrew_upper_chain (first :: middle ++ [last]) =
+    last :: upper_mid ++ [first] ->
+  Forall
+    (fun q =>
+       point_left_of_path_edges q (first :: rev upper_mid ++ [last]))
+    (first :: middle ++ [last]) ->
+  Forall
+    (fun q =>
+       point_left_of_path_edges q (last :: rev lower_mid ++ [first]))
+    (first :: middle ++ [last]) ->
+  is_max_hull'_edges
+    (andrew_hull (first :: middle ++ [last]))
+    (first :: middle ++ [last]).
+Proof.
+  intros first middle last lower_mid upper_mid Hsorted Hlower Hupper
+    Hupper_cover Hlower_cover.
+  unfold andrew_hull, andrew_merge.
+  assert (Hmerge :
+    andrew_ccw_merge
+      (first :: middle ++ [last])
+      (andrew_lower_chain (first :: middle ++ [last]))
+      (andrew_upper_chain (first :: middle ++ [last])) =
+      first :: lower_mid ++ last :: upper_mid).
+  {
+    eapply andrew_ccw_merge_endpoints; eauto.
+  }
+  rewrite Hmerge.
+  unfold is_max_hull'_edges.
+  rewrite Forall_forall in *.
+  intros q Hq.
+  destruct upper_mid as [| u upper_mid];
+  destruct lower_mid as [| l lower_mid].
+  - simpl.
+    assert (Hfirstq : leftdown first q).
+    {
+      simpl in Hq.
+      destruct Hq as [Hq | Hq].
+      - subst q.
+        apply leftdown_refl.
+      - simpl in Hsorted.
+        apply point_xy_sorted_from_leftdown_head in Hsorted.
+        rewrite Forall_forall in Hsorted.
+        apply Hsorted.
+        exact Hq.
+    }
+    assert (Hqlast : leftdown q last).
+    {
+      pose proof (point_xy_sorted_all_leftdown_last
+                    first middle last Hsorted) as Hall.
+      rewrite Forall_forall in Hall.
+      apply Hall.
+      exact Hq.
+    }
+    specialize (Hupper_cover q Hq) as Hupper_q.
+    specialize (Hlower_cover q Hq) as Hlower_q.
+    simpl in Hupper_q, Hlower_q.
+    destruct Hupper_q as [Hfl _].
+    destruct Hlower_q as [Hlf _].
+    eapply point_in_hull_edges_two_path_segment; eauto.
+  - replace (rev (first :: (l :: lower_mid) ++ last :: []))
+      with ([] ++ last :: rev (l :: lower_mid) ++ [first])
+      by (simpl; rewrite rev_app_distr; simpl;
+          repeat rewrite <- app_assoc; reflexivity).
+    change (point_in_hull_edges q
+      (rev (@nil point) ++ last :: rev (l :: lower_mid) ++ [first])).
+    eapply (point_in_hull_edges_andrew_merge_from_two_paths
+              q first (l :: lower_mid) last []).
+    + right; discriminate.
+    + apply Hupper_cover.
+      exact Hq.
+    + apply Hlower_cover.
+      exact Hq.
+  - replace (rev (first :: [] ++ last :: u :: upper_mid))
+      with (rev (u :: upper_mid) ++ last :: rev [] ++ [first]).
+    2: {
+      simpl.
+      repeat rewrite <- app_assoc.
+      reflexivity.
+    }
+    eapply (point_in_hull_edges_andrew_merge_from_two_paths
+              q first [] last (u :: upper_mid)).
+    + left; discriminate.
+    + apply Hupper_cover.
+      exact Hq.
+    + apply Hlower_cover.
+      exact Hq.
+  - replace (rev (first :: (l :: lower_mid) ++ last :: u :: upper_mid))
+      with (rev (u :: upper_mid) ++ last :: rev (l :: lower_mid) ++ [first]).
+    2: {
+      simpl.
+      rewrite rev_app_distr.
+      simpl.
+      repeat rewrite <- app_assoc.
+      reflexivity.
+    }
+    eapply (point_in_hull_edges_andrew_merge_from_two_paths
+              q first (l :: lower_mid) last (u :: upper_mid)).
+    + left; discriminate.
+    + apply Hupper_cover.
+      exact Hq.
+    + apply Hlower_cover.
+      exact Hq.
+Qed.
+
+Lemma andrew_hull_max_from_algorithmic_open_edge_covers :
+  forall sorted,
+  point_xy_sorted sorted ->
+  point_list_non_singleton sorted ->
+  (forall first middle last lower_mid upper_mid,
+    sorted = first :: middle ++ [last] ->
+    andrew_lower_chain sorted = first :: lower_mid ++ [last] ->
+    andrew_upper_chain sorted = last :: upper_mid ++ [first] ->
+    Forall
+      (fun q =>
+         point_left_of_path_edges q (first :: rev upper_mid ++ [last]))
+      sorted) ->
+  (forall first middle last lower_mid upper_mid,
+    sorted = first :: middle ++ [last] ->
+    andrew_lower_chain sorted = first :: lower_mid ++ [last] ->
+    andrew_upper_chain sorted = last :: upper_mid ++ [first] ->
+    Forall
+      (fun q =>
+         point_left_of_path_edges q (last :: rev lower_mid ++ [first]))
+      sorted) ->
+  is_max_hull'_edges (andrew_hull sorted) sorted.
+Proof.
+  intros sorted Hsorted Hnon Hupper_edges Hlower_edges.
+  destruct (point_list_non_singleton_first_last sorted Hnon)
+    as [first [middle [last Hshape]]].
+  subst sorted.
+  destruct (andrew_lower_chain_endpoints first middle last)
+    as [lower_mid Hlower].
+  destruct (andrew_upper_chain_endpoints first middle last)
+    as [upper_mid Hupper].
+  eapply andrew_hull_max_from_open_edge_covers.
+  - exact Hsorted.
+  - exact Hlower.
+  - exact Hupper.
+  - eapply Hupper_edges; eauto.
+  - eapply Hlower_edges; eauto.
 Qed.
 
 Lemma weak_rev_ccw_list_app_prefix :
@@ -2243,6 +4473,28 @@ Proof.
   exact Hweak.
 Qed.
 
+Lemma weak_rev_ccw_list_upper_fan_from_merged_convex :
+  forall first lower_mid last upper_mid,
+  leftmost first (lower_mid ++ last :: upper_mid) ->
+  ccw_convex (first :: lower_mid ++ last :: upper_mid) ->
+  weak_rev_ccw_list first (rev upper_mid ++ [last]).
+Proof.
+  intros first lower_mid last upper_mid Hleft Hconv.
+  destruct (ccw_convex_tail_sort_rev
+              first (lower_mid ++ last :: upper_mid) Hleft Hconv)
+    as [_ Hweak].
+  simpl in Hweak.
+  rewrite rev_app_distr in Hweak.
+  simpl in Hweak.
+  rewrite <- app_assoc in Hweak.
+  simpl in Hweak.
+  replace (rev upper_mid ++ last :: rev lower_mid)
+    with ((rev upper_mid ++ [last]) ++ rev lower_mid) in Hweak
+    by (rewrite <- app_assoc; reflexivity).
+  eapply weak_rev_ccw_list_app_prefix.
+  exact Hweak.
+Qed.
+
 Lemma lower_fan_covers_endpoints :
   forall first lower_mid last upper_mid,
   leftmost first (lower_mid ++ last :: upper_mid) ->
@@ -2259,6 +4511,106 @@ Proof.
     + exact Hweak.
   - apply gs_point_in_hull_new_head.
     exact Hweak.
+Qed.
+
+Lemma lower_fan_covers_member :
+  forall first lower_mid last upper_mid q,
+  leftmost first (lower_mid ++ last :: upper_mid) ->
+  ccw_convex (first :: lower_mid ++ last :: upper_mid) ->
+  In q lower_mid ->
+  point_in_hull q (first :: last :: rev lower_mid).
+Proof.
+  intros first lower_mid last upper_mid q Hleft Hconv Hq.
+  pose proof (weak_rev_ccw_list_lower_fan_from_merged_convex
+                first lower_mid last upper_mid Hleft Hconv) as Hweak.
+  apply point_in_hull_member_weak with (CH := last :: rev lower_mid).
+  - exact Hweak.
+  - simpl.
+    right.
+    apply (proj1 (in_rev lower_mid q)).
+    exact Hq.
+Qed.
+
+Lemma upper_fan_covers_member :
+  forall first lower_mid last upper_mid q,
+  leftmost first (lower_mid ++ last :: upper_mid) ->
+  ccw_convex (first :: lower_mid ++ last :: upper_mid) ->
+  In q upper_mid ->
+  point_in_hull q (first :: rev upper_mid ++ [last]).
+Proof.
+  intros first lower_mid last upper_mid q Hleft Hconv Hq.
+  pose proof (weak_rev_ccw_list_upper_fan_from_merged_convex
+                first lower_mid last upper_mid Hleft Hconv) as Hweak.
+  apply point_in_hull_member_weak with (CH := rev upper_mid ++ [last]).
+  - exact Hweak.
+  - rewrite in_app_iff.
+    left.
+    apply (proj1 (in_rev upper_mid q)).
+    exact Hq.
+Qed.
+
+Lemma upper_fan_covers_endpoints :
+  forall first lower_mid last upper_mid,
+  leftmost first (lower_mid ++ last :: upper_mid) ->
+  ccw_convex (first :: lower_mid ++ last :: upper_mid) ->
+  point_in_hull first (first :: rev upper_mid ++ [last]) /\
+  point_in_hull last (first :: rev upper_mid ++ [last]).
+Proof.
+  intros first lower_mid last upper_mid Hleft Hconv.
+  pose proof (weak_rev_ccw_list_upper_fan_from_merged_convex
+                first lower_mid last upper_mid Hleft Hconv) as Hweak.
+  split.
+  - apply gs_point_in_hull_anchor.
+    + destruct (rev upper_mid ++ [last]) as [| a rest] eqn:Hfan.
+      * apply app_eq_nil in Hfan as [_ Hlast_nil].
+        discriminate Hlast_nil.
+      * discriminate.
+    + exact Hweak.
+  - apply point_in_hull_last_weak.
+    exact Hweak.
+Qed.
+
+Lemma andrew_retained_point_two_fan_cover :
+  forall first middle last lower_mid upper_mid q,
+  point_xy_sorted (first :: middle ++ [last]) ->
+  andrew_lower_chain (first :: middle ++ [last]) =
+    first :: lower_mid ++ [last] ->
+  andrew_upper_chain (first :: middle ++ [last]) =
+    last :: upper_mid ++ [first] ->
+  In q lower_mid \/ In q upper_mid ->
+  point_in_hull q (first :: rev upper_mid ++ [last]) \/
+  point_in_hull q (first :: last :: rev lower_mid).
+Proof.
+  intros first middle last lower_mid upper_mid q
+    Hsorted Hlower Hupper Hretained.
+  assert (Hmerge :
+    andrew_ccw_merge
+      (first :: middle ++ [last])
+      (andrew_lower_chain (first :: middle ++ [last]))
+      (andrew_upper_chain (first :: middle ++ [last])) =
+      first :: lower_mid ++ last :: upper_mid).
+  {
+    eapply andrew_ccw_merge_endpoints; eauto.
+  }
+  assert (Hconv : ccw_convex (first :: lower_mid ++ last :: upper_mid)).
+  {
+    pose proof (andrew_hull_convex
+                  (first :: middle ++ [last]) Hsorted) as Hrevconv.
+    unfold andrew_hull, andrew_merge in Hrevconv.
+    rewrite Hmerge in Hrevconv.
+    apply gs_rev_ccw_convex_to_ccw_convex_rev in Hrevconv.
+    rewrite rev_involutive in Hrevconv.
+    exact Hrevconv.
+  }
+  assert (Hleft : leftmost first (lower_mid ++ last :: upper_mid)).
+  {
+    eapply andrew_ccw_merge_leftmost; eauto.
+  }
+  destruct Hretained as [Hlower_q | Hupper_q].
+  - right.
+    eapply lower_fan_covers_member; eauto.
+  - left.
+    eapply upper_fan_covers_member; eauto.
 Qed.
 
 Lemma andrew_two_fan_cover_of_middle :
@@ -2292,6 +4644,36 @@ Proof.
       * right.
         exact Hlast.
       * apply Forall_nil.
+Qed.
+
+Lemma andrew_two_fan_cover_from_side_covers :
+  forall first middle last lower_mid upper_mid,
+  Forall
+    (fun q =>
+       point_in_hull q (first :: last :: rev lower_mid) \/
+       ccw first last q)
+    middle ->
+  Forall
+    (fun q =>
+       point_in_hull q (first :: rev upper_mid ++ [last]) \/
+       ~ ccw first last q)
+    middle ->
+  Forall
+    (fun q =>
+       point_in_hull q (first :: rev upper_mid ++ [last]) \/
+       point_in_hull q (first :: last :: rev lower_mid))
+    middle.
+Proof.
+  intros first middle last lower_mid upper_mid Hlower Hupper.
+  rewrite Forall_forall in *.
+  intros q Hq.
+  specialize (Hlower q Hq) as [Hlower_q | Habove].
+  - right.
+    exact Hlower_q.
+  - specialize (Hupper q Hq) as [Hupper_q | Hnot_above].
+    + left.
+      exact Hupper_q.
+    + contradiction.
 Qed.
 
 Lemma andrew_hull_max_from_middle_two_fan_cover :
@@ -2356,21 +4738,110 @@ Proof.
   eapply andrew_merged_triangle_max_to_edges; eauto.
 Qed.
 
+Lemma andrew_chains_endpoints_coexist :
+  forall sorted,
+  point_list_non_singleton sorted ->
+  exists first middle last lower_mid upper_mid,
+    sorted = first :: middle ++ [last] /\
+    andrew_lower_chain sorted = first :: lower_mid ++ [last] /\
+    andrew_upper_chain sorted = last :: upper_mid ++ [first].
+Proof.
+  intros sorted Hnon.
+  destruct (point_list_non_singleton_first_last sorted Hnon)
+    as [first [middle [last Hsorted]]].
+  subst sorted.
+  destruct (andrew_lower_chain_endpoints first middle last)
+    as [lower_mid Hlower].
+  destruct (andrew_upper_chain_endpoints first middle last)
+    as [upper_mid Hupper].
+  exists first, middle, last, lower_mid, upper_mid.
+  repeat split; assumption.
+Qed.
+
+Lemma andrew_hull_max_from_algorithmic_two_fan_cover :
+  forall sorted,
+  point_xy_sorted sorted ->
+  point_list_non_singleton sorted ->
+  (forall first middle last lower_mid upper_mid,
+    sorted = first :: middle ++ [last] ->
+    andrew_lower_chain sorted = first :: lower_mid ++ [last] ->
+    andrew_upper_chain sorted = last :: upper_mid ++ [first] ->
+    Forall
+      (fun q =>
+         point_in_hull q (first :: rev upper_mid ++ [last]) \/
+         point_in_hull q (first :: last :: rev lower_mid))
+      middle) ->
+  is_max_hull'_edges (andrew_hull sorted) sorted.
+Proof.
+  intros sorted Hsorted Hnon Hcover.
+  destruct (andrew_chains_endpoints_coexist sorted Hnon)
+    as [first [middle [last [lower_mid [upper_mid
+       [Hshape [Hlower Hupper]]]]]]].
+  subst sorted.
+  eapply andrew_hull_max_from_middle_two_fan_cover.
+  - exact Hsorted.
+  - exact Hlower.
+  - exact Hupper.
+  - eapply Hcover; eauto.
+Qed.
+
+Lemma andrew_hull_max_from_algorithmic_side_covers :
+  forall sorted,
+  point_xy_sorted sorted ->
+  point_list_non_singleton sorted ->
+  (forall first middle last lower_mid upper_mid,
+    sorted = first :: middle ++ [last] ->
+    andrew_lower_chain sorted = first :: lower_mid ++ [last] ->
+    andrew_upper_chain sorted = last :: upper_mid ++ [first] ->
+    Forall
+      (fun q =>
+         point_in_hull q (first :: last :: rev lower_mid) \/
+         ccw first last q)
+      middle) ->
+  (forall first middle last lower_mid upper_mid,
+    sorted = first :: middle ++ [last] ->
+    andrew_lower_chain sorted = first :: lower_mid ++ [last] ->
+    andrew_upper_chain sorted = last :: upper_mid ++ [first] ->
+    Forall
+      (fun q =>
+         point_in_hull q (first :: rev upper_mid ++ [last]) \/
+         ~ ccw first last q)
+      middle) ->
+  is_max_hull'_edges (andrew_hull sorted) sorted.
+Proof.
+  intros sorted Hsorted Hnon Hlower Hupper.
+  eapply andrew_hull_max_from_algorithmic_two_fan_cover; eauto.
+  intros first middle last lower_mid upper_mid
+    Hshape Hlower_shape Hupper_shape.
+  eapply andrew_two_fan_cover_from_side_covers.
+  - eapply Hlower; eauto.
+  - eapply Hupper; eauto.
+Qed.
+
 Lemma andrew_hull_max_f : forall sorted,
   point_xy_sorted sorted ->
   point_list_non_singleton sorted ->
   is_max_hull'_edges (andrew_hull sorted) sorted.
 Proof.
-
-Abort.
+  intros sorted Hsorted Hnon.
+  eapply andrew_hull_max_from_algorithmic_open_edge_covers; eauto.
+  - intros first middle last lower_mid upper_mid
+      Hshape Hlower Hupper.
+    subst sorted.
+    eapply andrew_upper_chain_open_edge_cover; eauto.
+  - intros first middle last lower_mid upper_mid
+      Hshape Hlower Hupper.
+    subst sorted.
+    eapply andrew_lower_chain_open_edge_cover; eauto.
+Qed.
 
 Theorem andrew_hull_max : forall sorted,
   point_xy_sorted sorted ->
   point_list_non_singleton sorted ->
   is_max_hull'_edges (andrew_hull sorted) sorted.
 Proof.
-
-Abort.
+  exact andrew_hull_max_f.
+Qed.
 
 
 
